finished ex. 3, ex. 6 + updated type_infer

type_inferencer.lean
@@ -5,19 +5,6 @@ import .base_language
 Implement a type inferencer.
 -/
 
-def elam_helper : option ty → option ty
-| (some A) := some A
-| none := none
-
--- def eif_helper : option ty → option ty
--- | (some ty.TBool) :=
---     match if_branch_type, else_branch_type with
---     | (some A), (some B) := if (A = B) then (some A) else none
---     | _, _ := none
---     end
--- | _ := none
--- end
--- ℚ: No idea how to pattern match as an expression!
 
 def type_infer [decidable_eq ty] : ctx → exp → option ty
 | Γ (exp.EVar x) := ctx_lookup x Γ
@@ -26,7 +13,7 @@ def type_infer [decidable_eq ty] : ctx → exp → option ty
                                 (
                                     (
                                         λ output_type : option ty,
-                                            (elam_helper output_type)
+                                            bind (output_type) (λ o, some (ty.TFun A o))
                                     )
                                     (type_infer Γ' e)
                                 )
@@ -44,73 +31,66 @@ def type_infer [decidable_eq ty] : ctx → exp → option ty
                                 )
                         )
                         (ctx.ctx_snoc (ctx.ctx_snoc Γ x A) f (ty.TFun A B))
-| Γ (exp.EApp e1 e2) := let input_type : option ty := (type_infer Γ e2) in
-                        let output_type : option ty := (type_infer Γ e1) in
-                        match output_type with
-                        | (some (ty.TFun A B)) :=
-                            match input_type with
-                            | (some T) := if (A = T) then (some B) else none
-                            | _ := none
-                            end
-                        | _ := none
-                        end
+| Γ (exp.EApp e1 e2) :=
+    let input_type : option ty := (type_infer Γ e2) in
+    let output_type : option ty := (type_infer Γ e1) in
+    match output_type with
+    | (some (ty.TFun A B)) :=
+        match input_type with
+        | (some T) := if (A = T) then (some B) else none
+        | _ := none
+        end
+    | _ := none
+    end
 | Γ (exp.ETrue) := some ty.TBool
 | Γ (exp.EFalse) := some ty.TBool
-| Γ (exp.EIf e1 e2 e3) := let cond_type : option ty := (type_infer Γ e1) in
-                          let if_branch_type : option ty := (type_infer Γ e2) in
-                          let else_branch_type : option ty := (type_infer Γ e3) in
-                          match cond_type with
-                          | (some ty.TBool) :=
-                              match if_branch_type, else_branch_type with
-                              | (some A), (some B) := if (A = B) then (some A) else none
-                              | _, _ := none
-                              end
-                          | _ := none
-                          end
-                          /-
-                          Alternative:
-                          (
-                            λ cond_type : option ty,
-                                (
-                                    (
-                                        λ if_branch_type : option ty,
-                                            (
-                                                (
-                                                    λ else_branch_type : option ty,
-                                                        (
-                                                            eif_helper
-                                                        )
-                                                )
-                                                (type_infer Γ e3)
-                                            )
-                                    )
-                                    (type_infer Γ e2)
-                                )
-                          ) 
-                          ((type_infer Γ e1))
-                          -/
+| Γ (exp.EIf e1 e2 e3) :=
+    bind (type_infer Γ e1)
+    (λ cond_type,
+        if (cond_type = ty.TBool)
+        then (
+            bind (type_infer Γ e2)
+            (λ if_branch_type,
+                bind (type_infer Γ e3)
+                (λ else_branch_type,
+                    if (if_branch_type = else_branch_type)
+                    then some if_branch_type
+                    else none
+                )
+            )
+        )
+        else none
+    )
 | Γ (exp.Ezero) := some ty.TNat
 | Γ (exp.ESucc) := some (ty.TFun ty.TNat ty.TNat)
 | Γ (exp.EPred) := some (ty.TFun ty.TNat ty.TNat)
 | Γ (exp.EIsZero) := some (ty.TFun ty.TNat ty.TBool)
-| Γ (exp.EPair e1 e2) := let l_type : option ty := (type_infer Γ e1) in
-                         let r_type : option ty := (type_infer Γ e2) in
-                         match l_type, r_type with
-                         | (some A), (some B) := some (ty.TProd A B)
-                         | _, _ := none
-                         end
-| Γ (exp.EFst e) := let pair_type : option ty := (type_infer Γ e) in
-                    match pair_type with
-                    | some (ty.TProd A B) := some A
-                    | _ := none
-                    end
-| Γ (exp.ESnd e) := let pair_type : option ty := (type_infer Γ e) in
-                    match pair_type with
-                    | some (ty.TProd A B) := some B
-                    | _ := none
-                    end
+| Γ (exp.EPair e1 e2) :=
+    let l_type : option ty := (type_infer Γ e1) in
+    let r_type : option ty := (type_infer Γ e2) in
+    match l_type, r_type with
+    | (some A), (some B) := some (ty.TProd A B)
+    | _, _ := none
+    end
+| Γ (exp.EFst e) := 
+    let pair_type : option ty := (type_infer Γ e) in
+    match pair_type with
+    | some (ty.TProd A B) := some A
+    | _ := none
+    end
+| Γ (exp.ESnd e) := 
+    let pair_type : option ty := (type_infer Γ e) in
+    match pair_type with
+    | some (ty.TProd A B) := some B
+    | _ := none
+    end
 ------------
 
 -- Sanity check:
 #eval type_infer (ctx.ctx_nil) (exp.ELam "x" ty.TNat (exp.EIsZero))
 #eval some $ ty.TFun ty.TNat (ty.TFun ty.TNat ty.TBool)
+
+#eval type_infer (ctx.ctx_nil) (exp.EIf exp.ETrue exp.EFalse exp.ETrue)
+#eval some $ ty.TBool
+
+#eval type_infer (ctx.ctx_nil) (exp.EIf exp.ETrue exp.Ezero exp.ETrue)
