exercise_6.lean
@@ -5,19 +5,20 @@ import .base_language .type_inferencer
 -/
 
 -- Define some standard contexts:
+def f : string := "f"
 def x : string := "x"
 def Γ₀ : ctx := ctx.ctx_nil
 def Γ₁ : ctx := ctx.ctx_snoc Γ₀ x ty.TNat 
 
 -- Positive tests:
-def legal₁_exp : exp := exp.ELam "x" ty.TNat (exp.EIsZero)
+def legal₁_exp : exp := exp.ELam x ty.TNat (exp.EIsZero)
 lemma legal₁ : (type_infer Γ₀ legal₁_exp) = some (ty.TFun ty.TNat (ty.TFun ty.TNat ty.TBool)) :=
   begin
     unfold Γ₀,
     unfold legal₁_exp,
     unfold type_infer,
-    unfold elam_helper,
-    sorry -- This does not look right (Is there a mistake in the type checker definition?)
+    unfold bind,
+    exact rfl
   end
 
 def legal₂_exp : exp := (exp.ELam x ty.TNat (exp.EVar x))
@@ -26,14 +27,43 @@ lemma legal₂ : (type_infer Γ₀ legal₂_exp) = (ty.TFun ty.TNat ty.TNat) :=
     unfold Γ₀,
     unfold legal₂_exp,
     unfold type_infer,
-    sorry
+    unfold bind,
+    exact rfl
   end
 
-def legal₃_exp : exp := sorry
-lemma legal₃ : (type_infer Γ₁ legal₃_exp) = sorry := sorry
+def legal₃_exp : exp := exp.ERec
+      f
+      x
+      ty.TNat
+      ty.TNat
+      (
+        exp.EIf
+          (exp.EApp exp.EIsZero (exp.EVar x))
+          exp.Ezero
+          (
+            exp.EApp
+              exp.ESucc
+              (
+                exp.EApp
+                  exp.ESucc
+                  (exp.EApp (exp.EVar f) (exp.EApp exp.EPred (exp.EVar x)))
+              )
+          )
+      )
+lemma legal₃ : (type_infer Γ₁ legal₃_exp) = ty.TFun ty.TNat ty.TNat :=
+  begin
+    unfold Γ₁,
+    unfold legal₃_exp,
+    unfold type_infer,
+    unfold bind,
+    exact rfl
+  end
 
-def legal₄_exp : exp := sorry
-lemma legal₄ : (type_infer Γ₁ legal₄_exp) = sorry := sorry
+def legal₄_exp : exp := exp.EApp exp.ESucc exp.Ezero
+lemma legal₄ : (type_infer Γ₁ legal₄_exp) = ty.TNat :=
+  begin
+    exact rfl
+  end
 
 -- Negative tests:
 -- Illegal test 1 ⇒ if 0 then 'true' else 'false'
@@ -42,8 +72,12 @@ lemma illegal₁ : (type_infer ctx.ctx_nil illegal₁_exp) = none :=
   begin
     unfold illegal₁_exp,
     unfold type_infer,
-    sorry
+    unfold bind,
+    exact rfl
   end
 
-def illegal₂_exp : exp := sorry
-lemma illegal₂ : (type_infer Γ₀ illegal₂_exp) = none := sorry
+def illegal₂_exp : exp := exp.EApp (exp.ELam x ty.TNat exp.ESucc) exp.ETrue
+lemma illegal₂ : (type_infer Γ₀ illegal₂_exp) = none :=
+  begin
+    exact rfl
+  end
